requisiteness with non-trivial postcondition, thanks Johannes

theories/program_logic/requisiteness.v
@@ -38,10 +38,10 @@ Global Arguments stateful_pure {_ _ _ _ _} _%_stdpp_scope.
 Notation "⌞ P ⌟" := (stateful_pure P) (format "⌞ P ⌟") : bi_scope.
 
 Class requisiteG Λ Σ := RequisiteG {
-  #[local] requisiteG_bag :: ghost_mapG Σ nat (expr Λ);
+  #[local] requisiteG_bag :: ghost_mapG Σ nat (expr Λ * (val Λ → Prop));
 }.
 
-Definition requisiteΣ Λ := #[ghost_mapΣ nat (expr Λ)].
+Definition requisiteΣ Λ := #[ghost_mapΣ nat (expr Λ * (val Λ → Prop))].
 
 Global Instance subG_requisiteG Λ Σ :
   subG (requisiteΣ Λ) Σ → requisiteG Λ Σ.
@@ -51,16 +51,17 @@ Section requisiteness.
   Context `{!irisGS_gen hlc Λ Σ, !coirisG_gen hlc Λ Σ, !requisiteG Λ Σ}.
 
   Implicit Types (e : expr Λ) (v : val Λ) (σ : state Λ) (t : list (expr Λ)) (Q : (val Λ) → (state Λ) → Prop).
-  Notation safe_tp s t1 σ1 := (∀ t2 σ2 e2, s = NotStuck →
-    rtc erased_step (t1, σ1) (t2, σ2) → e2 ∈ t2 → not_stuck e2 σ2).
 
   Local Instance into_val_val v : IntoVal (of_val v) v.
   Proof. done. Qed.
 
-  Definition safeInv γb : iProp Σ :=
+  Definition add_postcond (φ : val Λ → Prop) (t : list (expr Λ)) :=
+    zip t (φ :: repeat (λ _, True) (length t - 1)).
+
+  Definition requisiteInv φ γb : iProp Σ :=
     ∃ t2 σl nsl κsl ntl, own_state σl nsl κsl ntl ∗
-      ghost_map_auth γb 1 (list_to_map (zip (seq 0 (length t2)) t2)) ∗
-      ⌜safe_tp NotStuck t2 σl ⌝.
+      ghost_map_auth γb 1 (list_to_map (zip (seq 0 (length t2)) (add_postcond φ t2))) ∗
+      ⌜adequate_tp NotStuck t2 σl (λ v _, φ v)⌝.
 
   (* TOOD: move to stdpp *)
   Local Lemma zip_cons {A B} (a : A) (l : list A) (b : B) (k : list B) :
@@ -76,38 +77,61 @@ Section requisiteness.
       rewrite list_lookup_fmap. by destruct (zip l k !! i) as [[??]|]. }
     rewrite {1}Hidf -zip_with_zip zip_with_app //.
   Qed.
+  Local Lemma repeat_S {A} (a : A) n :
+    repeat a (S n) = a::repeat a n.
+  Proof. done. Qed.
 
-  Local Lemma wptp_weak_requisiteness_inv t γb :
-    inv nroot (safeInv γb) ⊢
-    [∗ list] e ∈ t, (∃ i, i ↪[γb] e) -∗ WP e {{ _, True }}.
+  Local Lemma wptp_requisiteness_inv (tφ : list (expr Λ * (val Λ → Prop))) φ₀ γb :
+    inv nroot (requisiteInv φ₀ γb) ⊢
+    [∗ list] eφ ∈ tφ, (∃ i, i ↪[γb] eφ) -∗ let '(e,φ) := eφ in WP e {{ v, ⌜φ v⌝ }}.
   Proof.
+    pose (Truep := λ _ : val Λ, True).
     iIntros "#Hinv".
-    iLöb as "IH" forall (t).
+    iLöb as "IH" forall (tφ).
     iApply (big_sepL_impl (λ _ _, emp)%I); first done.
-    iIntros "!#" (? e _) "_ [%tid He◯]".
+    iIntros "!#" (? [e φ] _) "_ [%tid He◯]".
     destruct (to_val e) as [v|] eqn:He.
 
     - rewrite -(of_to_val e v); last apply He.
-      by iApply wp_value.
+      iApply wp_value_fupd.
+      iInv nroot as "H" "Hclose".
+      (* TODO: is there a way to provide an IntoExist instance under ◇ modality? *)
+      iDestruct (bi.later_exist_except_0 with "H") as ">[%t1 H]".
+      iDestruct (bi.later_exist_except_0 with "H") as ">[%σl1 H]".
+      iDestruct (bi.later_exist_except_0 with "H") as ">[%nsl H]".
+      iDestruct (bi.later_exist_except_0 with "H") as ">[%κl H]".
+      iDestruct (bi.later_exist_except_0 with "H") as ">[%ntl H]".
+      iDestruct "H" as ">(Hown_state & Ht● & %Hadq)".
+      iDestruct (ghost_map_lookup with "Ht● He◯") as %Hint1%elem_of_list_to_map_2%elem_of_zip_r.
+      iMod ("Hclose" with "[$Hown_state $Ht● //]") as "_".
+      iPureIntro.
+      destruct Hadq.
+      destruct t1 as [|e1 t1]; first done.
+      rewrite /add_postcond zip_cons length_cons elem_of_cons in Hint1.
+      replace (S (length t1) -1) with (length t1) in Hint1 by lia.
+      destruct Hint1 as [Hmain_thread | Hint1].
+      + simplify_eq. eapply adequate_tp_result, rtc_refl.
+      + apply elem_of_zip_r, list_elem_of_In, repeat_spec in Hint1.
+        rewrite Hint1 //.
 
     - iApply wp_lift_step_fupd; first done.
       iIntros (σ1 ns κ κs nt) "Hstate_interp".
-      (* TODO: is there a way to provide an IntoExist instance under ◇ modality? *)
       iInv nroot as "H" "Hclose1".
       iDestruct (bi.later_exist_except_0 with "H") as ">[%t1 H]".
       iDestruct (bi.later_exist_except_0 with "H") as ">[%σl1 H]".
       iDestruct (bi.later_exist_except_0 with "H") as ">[%nsl H]".
       iDestruct (bi.later_exist_except_0 with "H") as ">[%κl H]".
       iDestruct (bi.later_exist_except_0 with "H") as ">[%ntl H]".
-      iDestruct "H" as ">(Hown_state & Ht● & %Hsafe)".
+      iDestruct "H" as ">(Hown_state & Ht● & %Hadq)".
       iApply fupd_mask_intro; first set_solver. iIntros "Hclose2".
       iDestruct (own_state_agree with "Hstate_interp Hown_state") as %Hσlσ.
       iDestruct (ghost_map_lookup with "Ht● He◯") as %Hint1%elem_of_list_to_map_2.
 
       assert (He_red : reducible e σl1). {
-        specialize (Hsafe t1 σl1 e).
-        destruct Hsafe as [Hfalse|]; try done.
-        - by eapply elem_of_zip_r.
+        destruct Hadq.
+        specialize (adequate_tp_not_stuck t1 σl1 e eq_refl (ltac:(apply rtc_refl))).
+        destruct adequate_tp_not_stuck as [Hfalse|]; try done.
+        - by eapply elem_of_zip_l,elem_of_zip_r.
         - rewrite /= He in Hfalse. by inversion Hfalse.
       }
 
@@ -115,23 +139,27 @@ Section requisiteness.
       iIntros (e2 σ2 efs Hprim_step) "_ !>!>".
 
       (* update ghost resources *)
-      iMod (ghost_map_update e2 with "Ht● He◯") as "[Ht● He◯]".
-      iMod (ghost_map_insert_big (list_to_map (zip (seq (length t1) (length efs)) efs)) with "Ht●") as "[Ht● Hefs◯]".
+      iMod (ghost_map_update (e2, φ) with "Ht● He◯") as "[Ht● He◯]".
+      iMod (ghost_map_insert_big (list_to_map (zip (seq (length t1) (length efs)) (zip efs (repeat Truep (length efs))))) with "Ht●") as "[Ht● Hefs◯]".
       { apply map_disjoint_dom.
-        rewrite dom_insert_L !dom_list_to_map_L !fst_zip; [|by rewrite length_seq..].
+        rewrite dom_insert_L !dom_list_to_map_L !fst_zip; first last.
+        { rewrite length_seq length_zip repeat_length. lia. }
+        { rewrite length_seq length_zip length_cons repeat_length. lia. }
         rewrite !list_to_set_seq.
         assert (tid ∈ (set_seq 0 (length t1) : gset nat)).
         { eapply elem_of_set_seq, elem_of_seq, elem_of_zip_l => //. }
         replace ({[tid]} ∪ set_seq 0 (length t1) : gset nat) with (set_seq 0 (length t1) : gset nat) by set_solver.
         symmetry. apply set_seq_add_disjoint. }
-      iAssert ([∗ list] i↦k ∈ efs, (length t1+i) ↪[γb] k)%I with "[Hefs◯]" as "Hefs◯".
+      iAssert ([∗ list] i↦'(k,φ) ∈ (zip efs (repeat Truep (length efs))), (length t1+i) ↪[γb] (k,φ))%I with "[Hefs◯]" as "Hefs◯".
       { clear.
         remember (length t1) as len. clear Heqlen.
         iInduction efs as [|ef efs] "IHf" forall (len); first done.
-        rewrite big_sepL_cons length_cons -cons_seq zip_cons list_to_map_cons big_sepM_insert; last first.
+        rewrite length_cons repeat_S zip_cons big_sepL_cons.
+        rewrite -cons_seq zip_cons list_to_map_cons big_sepM_insert; last first.
         { apply not_elem_of_dom_1.
-          rewrite dom_list_to_map_L fst_zip; last by rewrite length_seq.
-          rewrite list_to_set_seq elem_of_set_seq. lia. }
+          rewrite dom_list_to_map_L fst_zip.
+          - rewrite list_to_set_seq elem_of_set_seq. lia.
+          - rewrite length_seq length_zip repeat_length. lia. }
         rewrite right_id.
         iDestruct "Hefs◯" as "[$ Hefs◯]".
         iDestruct ("IHf" with "Hefs◯") as "Hefs◯".
@@ -148,10 +176,16 @@ Section requisiteness.
       iMod "Hclose2" as "_".
       iMod ("Hclose1" with "[Ht● $Hown_state]") as "_".
       { (* destruct [t1] into [t1a++e::t1b] *)
-        assert (Hlookupt1: t1!!tid = Some e).
+        assert (Hlen_add_postcond_φ₀_t1: length t1 = length (add_postcond φ₀ t1)).
+        { destruct t1; first set_solver.
+          rewrite /add_postcond zip_cons !length_cons length_zip repeat_length. lia. }
+        rewrite Hlen_add_postcond_φ₀_t1 in Hint1.
+        rewrite Hlen_add_postcond_φ₀_t1.
+        remember (add_postcond φ₀ t1) as t1φ.
+        assert (Hlookupt1φ: t1φ!!tid = Some (e,φ)).
         { clear -Hint1.
-          assert (lemma: ∀ i, (tid,e) ∈ zip (seq i (length t1)) t1 → i≤tid ∧ t1 !! (tid-i) = Some e).
-          { clear. induction t1 as [|e0 t1 IH] => i Hint1; first set_solver.
+          assert (lemma: ∀ i, (tid,(e,φ)) ∈ zip (seq i (length t1φ)) t1φ → i≤tid ∧ t1φ !! (tid-i) = Some (e,φ)).
+          { clear. induction t1φ as [|e0 t1φ IH] => i Hint1; first set_solver.
             rewrite /= elem_of_cons in Hint1. destruct Hint1 as [Hint1|Hint1].
             - simplify_eq. replace (i-i) with 0 by lia. set_solver.
             - destruct (IH _ Hint1) as [Hle Hlookupt1].
@@ -162,83 +196,139 @@ Section requisiteness.
           destruct (lemma 0 Hint1) as [_ H].
           replace (tid-0) with (tid) in H by lia.
           done. }
-        destruct (list_elem_of_split_length t1 tid e Hlookupt1) as (t1a & t1b & -> & ->).
+        destruct (list_elem_of_split_length t1φ tid (e,φ) Hlookupt1φ) as (t1φa & t1φb & -> & ->).
 
         (* update [e] to [e2] *)
-        iEval (rewrite [x in seq 0 x]length_app seq_app) in "Ht●".
-        iEval (rewrite zip_app; last rewrite length_seq //) in "Ht●".
-        iEval (rewrite length_cons -cons_seq zip_cons) in "Ht●".
-        assert ((list_to_map (zip (seq 0 (length t1a)) t1a) : gmap nat (expr Λ)) !! length t1a = None).
-        { apply not_elem_of_dom_1.
-          rewrite dom_list_to_map_L fst_zip; last by rewrite length_seq.
-          rewrite list_to_set_seq elem_of_set_seq.
-          lia. }
-        iEval (rewrite list_to_map_app list_to_map_cons -(insert_union_r _ _ (length t1a) e) //) in "Ht●".
-        iEval (rewrite insert_insert_eq) in "Ht●".
-        iEval (rewrite (insert_union_r _ _ (length t1a) e2) //) in "Ht●".
-        iEval (rewrite -list_to_map_cons -list_to_map_app) in "Ht●".
-        iEval (rewrite -zip_cons cons_seq -(length_cons e2)) in "Ht●".
-        iEval (rewrite -zip_app; last by apply length_seq) in "Ht●".
-        iEval (rewrite -seq_app -[x in seq 0 x]length_app) in "Ht●".
+        replace (<[length t1φa:=(e2, φ)]> (
+          list_to_map (zip (seq 0 (length (t1φa ++ (e,φ) :: t1φb)))
+          (t1φa ++ (e,φ) :: t1φb))))
+          with (list_to_map (zip (seq 0 (length (t1φa ++ (e2,φ) :: t1φb)))
+          (t1φa ++ (e2,φ) :: t1φb)) : gmap _ _); last first.
+        { rewrite !length_app !seq_app.
+          rewrite !zip_app; [|by rewrite length_seq..].
+          rewrite !length_cons -!cons_seq !zip_cons.
+          assert ((list_to_map (zip (seq 0 (length t1φa)) t1φa) : gmap _ _) !! length t1φa = None).
+          { apply not_elem_of_dom_1.
+            rewrite dom_list_to_map_L fst_zip; last by rewrite length_seq.
+            rewrite list_to_set_seq elem_of_set_seq.
+            lia. }
+          rewrite !list_to_map_app !list_to_map_cons -!insert_union_r //.
+          rewrite insert_insert_eq //. }
 
-        replace (length (t1a++e::t1b)) with (length (t1a++e2::t1b));
+        replace (length (t1φa++(e,φ)::t1φb)) with (length (t1φa++(e2,φ)::t1φb));
           last rewrite !length_app //.
 
         (* merge two [list_to_map]s *)
         rewrite map_union_comm; last first.
         { apply map_disjoint_dom.
-          rewrite !dom_list_to_map_L !fst_zip; [|by rewrite length_seq..].
+          rewrite !dom_list_to_map_L !fst_zip; first last.
+          { rewrite length_seq length_zip repeat_length. lia. }
+          { rewrite length_seq. lia. }
           rewrite !list_to_set_seq.
           apply elem_of_disjoint => tid Hin1 Hin2.
           apply elem_of_set_seq in Hin1,Hin2.
           lia. }
         iEval (rewrite -list_to_map_app -zip_app; last by rewrite length_seq) in "Ht●".
-        iEval (rewrite -[x in seq x (length efs)](left_id 0 Nat.add (length (t1a++e2::t1b)))) in "Ht●".
-        iEval (rewrite -seq_app -length_app) in "Ht●".
-        rewrite -assoc -app_comm_cons.
+        iEval (rewrite -seq_app) in "Ht●".
+        replace (length (t1φa ++ (e2, φ) :: t1φb) + length efs)
+          with (length (t1φa.*1++e2::t1φb.*1++efs)); last first.
+        { rewrite !length_app !length_cons length_app !length_fmap. lia. }
+        replace ((t1φa ++ (e2, φ) :: t1φb) ++ zip efs (repeat Truep (length efs)))
+          with (add_postcond φ₀ (t1φa.*1++e2::t1φb.*1++efs)); last first.
+        { rewrite /add_postcond in Heqt1φ.
+          apply (f_equal (λ x, x.*2)) in Heqt1φ.
+          rewrite snd_zip in Heqt1φ; last first.
+          { destruct t1.
+            - rewrite length_nil length_app length_cons in Hlen_add_postcond_φ₀_t1.
+              lia.
+            - rewrite !length_cons repeat_length. lia. }
+          rewrite fmap_app fmap_cons /= in Heqt1φ.
+          rewrite /add_postcond.
+          replace (length (t1φa.*1 ++ e2 :: t1φb.*1 ++ efs) - 1)
+            with (length t1 - 1 + length efs); last first.
+          { rewrite Hlen_add_postcond_φ₀_t1.
+            rewrite !length_app !length_cons length_app !length_fmap. lia. }
+          rewrite repeat_app [x in zip _ x]app_comm_cons -Heqt1φ.
+          rewrite [in x in zip x _]app_comm_cons assoc zip_app;
+            last by rewrite !length_app !length_cons !length_fmap.
+          f_equal.
+          rewrite -[x in _ = x]zip_fst_snd !fmap_app !fmap_cons //. }
 
         iFrame "Ht●". iIntros "!>!%".
-        intros t3 σ3 e3 _ Hsteps.
-        apply Hsafe; first done.
-        eapply rtc_l; last exact Hsteps.
-        exists κ.
-        by apply (step_atomic e σl1 e2 σl2 efs t1a t1b). }
+        rewrite /add_postcond in Heqt1φ.
+        apply (f_equal (λ x, x.*1)) in Heqt1φ.
+        rewrite fst_zip in Heqt1φ; last (rewrite length_cons repeat_length; lia).
+        rewrite fmap_app fmap_cons /= in Heqt1φ.
+        rewrite -Heqt1φ in Hadq.
+        eapply adequate_tp_erased_step; last exact Hadq.
+        exists κ. by eapply step_atomic. }
 
-      iModIntro. simpl.
-      iAssert (∃ tid, tid ↪[γb] e2)%I with "[$He◯]" as "He◯".
-      iDestruct (big_sepL_mono _ (λ _ e, ∃ i, i ↪[γb] e)%I with "Hefs◯") as "Hefs◯".
-      { iIntros (???) "$". }
+      iModIntro.
+      iAssert (∃ tid, tid ↪[γb] (e2, φ))%I with "[$He◯]" as "He◯".
+      iDestruct (big_sepL_mono _ (λ _ eφ, ∃ i, i ↪[γb] eφ)%I with "Hefs◯") as "Hefs◯".
+      { iIntros (? [? ?] ?) "$". }
       iCombine "He◯ Hefs◯" as "Ht◯".
-      rewrite -(big_sepL_cons (λ _ e, ∃ i, i ↪[γb] e)%I).
-      rewrite -(big_sepL_mono (λ _ e, WP e {{_, True}})%I ((λ _ e, WP e {{fork_post}})%I)); last first.
+      rewrite -(big_sepL_cons (λ _ eφ, ∃ i, i ↪[γb] eφ)%I).
+      pose (f:=(λ e, (e,Truep))).
+      replace (zip efs (repeat Truep (length efs))) with (f <$> efs); last first.
+      { clear. induction efs; first done.
+        rewrite fmap_cons length_cons repeat_S zip_cons. f_equal. assumption. }
+      pose (Φ := (λ (_ : nat) '(e,φ), WP e {{v, ⌜φ v⌝}})%I).
+      rewrite -(big_sepL_mono (λ i e, Φ i (f e))%I ((λ _ e, WP e {{fork_post}})%I)); last first.
       { intros ???. apply wp_mono =>?. iIntros "_". iApply fork_post_trivial. }
-      rewrite -(big_sepL_cons (λ _ e, WP e {{_, True}})%I).
-      iApply (big_sepL_wand with "Ht◯").
+      rewrite -(big_sepL_fmap f Φ). rewrite /Φ /f.
+      rewrite -(big_sepL_cons Φ (e2,φ)).
+      iApply (big_sepL_wand with "Ht◯"). rewrite /Φ.
       iApply "IH".
   Qed.
 
-  Lemma wptp_weak_requisiteness t P :
-    (∀ σ, P σ → safe_tp NotStuck t σ) →
-    ⌞P⌟ ⊢ |={⊤}=> [∗ list] e ∈ t, WP e {{ _, True }}.
+  Lemma wptp_requisiteness e t φ P :
+    (∀ σ, P σ → adequate_tp NotStuck (e::t) σ (λ v _, φ v)) →
+    ⌞P⌟ ⊢ |={⊤}=> WP e {{ v, ⌜φ v⌝ }} ∗ [∗ list] e ∈ t, WP e {{ _, True }}.
   Proof.
-    iIntros (Hsafe) "HP".
+    iIntros (Hadq) "HP".
     iDestruct "HP" as (σl nsl κsl ntl) "[Hown_state %HP]".
-    specialize (Hsafe σl HP).
-    iMod (ghost_map_alloc (list_to_map (zip (seq 0 (length t)) t))) as (γb) "[Ht● Ht◯]".
-    iAssert ([∗ list] k ∈ t, ∃ i, i ↪[γb] k)%I with "[Ht◯]" as "Ht◯".
+    specialize (Hadq σl HP).
+    iMod (ghost_map_alloc (list_to_map (zip (seq 0 (length (e::t))) (add_postcond φ (e::t))))) as (γb) "[Ht● Ht◯]".
+    iAssert ([∗ list] k ∈ add_postcond φ (e::t), ∃ i, i ↪[γb] k)%I with "[Ht◯]" as "Ht◯".
     { clear.
       remember 0 as start. clear Heqstart.
-      iInduction t as [|e t] "IH" forall (start); first done.
+      replace (length (e::t)) with (length (add_postcond φ (e::t))); last first.
+      { rewrite /add_postcond zip_cons !length_cons length_zip repeat_length. lia. }
+      remember (add_postcond φ (e::t)) as tφ. clear Heqtφ.
+      iInduction tφ as [|eφ tφ] "IH" forall (start); first done.
       rewrite big_sepL_cons length_cons -cons_seq zip_cons list_to_map_cons big_sepM_insert; last first.
       { apply not_elem_of_dom_1.
         rewrite dom_list_to_map_L fst_zip; last by rewrite length_seq.
         rewrite list_to_set_seq elem_of_set_seq. lia. }
       iDestruct "Ht◯" as "[$ Ht◯]".
       by iApply "IH". }
-    iMod (inv_alloc nroot ⊤ (safeInv γb) with "[$Hown_state $Ht● //]") as "#Hinv".
+    iMod (inv_alloc nroot ⊤ (requisiteInv φ γb) with "[$Hown_state $Ht● //]") as "#Hinv".
+
     iModIntro.
+    pose (f:=(λ e, (e, λ v, True))).
+    rewrite /add_postcond zip_cons.
+    replace (zip t (repeat (λ v, True) (length (e::t) - 1))) with (f <$> t); last first.
+    { clear.
+      replace (length (e::t)-1) with (length t) by (rewrite length_cons; lia).
+      induction t; first done.
+      rewrite fmap_cons length_cons repeat_S zip_cons. f_equal. assumption. }
+    pose (Φ := (λ (_ : nat) '(e,φ), WP e {{v, ⌜φ v⌝}})%I).
+    rewrite -(big_sepL_mono (λ i e, Φ i (f e))%I ((λ _ e, WP e {{_, True}})%I)); last first.
+    { intros ???. apply wp_mono =>? //. }
+    rewrite -(big_sepL_fmap f Φ). rewrite /Φ /f.
+    rewrite -(big_sepL_cons Φ (e,φ)). rewrite /Φ.
     iApply (big_sepL_wand with "Ht◯").
-    by iApply wptp_weak_requisiteness_inv.
+    by iApply wptp_requisiteness_inv.
+  Qed.
+
+  Lemma wp_requisiteness e φ P :
+    (∀ σ, P σ → adequate NotStuck e σ (λ v _, φ v)) →
+    ⌞P⌟ ⊢ WP e {{ v, ⌜φ v⌝ }}.
+  Proof.
+    iIntros (Hadq) "HP".
+    iMod (wptp_requisiteness e [] with "HP") as "[$ _]".
+    intros σ HP. apply adequate_tp_adequate. auto.
   Qed.
 
   Lemma wp_requisiteness_nofork e P Q :
@@ -343,10 +433,4 @@ Section requisiteness.
     eapply adequate_nofork_prim_step; first exact Hprim_step_l.
     assumption.
   Qed.
-
-  (* False *)
-  Lemma wptp_requisiteness e t P Q :
-    (∀ σ, P σ → adequate_tp NotStuck (e::t) σ Q) →
-    ⌞P⌟ ⊢ |={⊤}=> WP e {{ v, ⌞Q v⌟ }} ∗ [∗ list] e ∈ t, WP e {{ _, True }}.
-  Abort.
 End requisiteness.
